SystemF/Typing.lean
@@ -9,19 +9,19 @@ namespace SystemF
 inductive HasType : Context → Tm → Ty → Prop where
   | var Γ x T :
     WfContext Γ →
-    (x, T) ∈ Γ →
+    (x, .tm T) ∈ Γ →
     LcTy T →
     HasType Γ ($v x) T
   | lam (L : Finset Name) Γ T₁ T₂ t :
     LcTy T₁ →
-    (∀ x ∉ L, HasType ((x, T₁) :: Γ) (t⟪$v x⟫) T₂) →
+    (∀ x ∉ L, HasType ((x, .tm T₁) :: Γ) (t⟪$v x⟫) T₂) →
     HasType Γ (ƛ T₁ => t) (T₁ ⇒ T₂)
   | app Γ t₁ t₂ T₁ T₂ :
     HasType Γ t₁ (T₁ ⇒ T₂) →
     HasType Γ t₂ T₁ →
     HasType Γ (t₁ ◦ t₂) T₂
   | tLam (L : Finset Name) Γ t T :
-    (∀ X ∉ L, HasType Γ (t⟪$T X⟫) (T⟪$T X⟫)) →
+    (∀ X ∉ L, HasType ((X, .ty) :: Γ) (t⟪$T X⟫) (T⟪$T X⟫)) →
     HasType Γ (Λ' t) (∀' T)
   | tApp Γ t T₁ T₂ :
     HasType Γ t (∀' T₁) →
@@ -34,7 +34,11 @@ scoped notation Γ " ⊢ " t " ∶ " T => HasType Γ t T
   Substituting free variable `X` with `U` in a context `Γ` (all types in `Γ` are substituted).
 -/
 def substCtx (X : Name) (U : Ty) (Γ : Context) : Context :=
-  Γ.map (fun ⟨y, T⟩ => (y, substTy X U T))
+  Γ.map (fun ⟨y, b⟩ =>
+    match b with
+    | .ty => (y, .ty)
+    | .tm T => (y, .tm (substTy X U T))
+  )
 
 @[simp]
 instance : Subst Ty Context where
@@ -44,8 +48,12 @@ instance : Subst Ty Context where
 lemma substCtx_nil {X : Name} {U : Ty} : ([][X ↦ U] : Context) = [] := rfl
 
 @[simp]
-lemma substCtx_cons {Γ : Context} {X : Name} {U : Ty} {y : Name} {T : Ty} :
-   ((y, T) :: Γ)[X ↦ U] = (y, T[X ↦ U]) :: Γ[X ↦ U] := rfl
+lemma substCtx_cons_tm {Γ : Context} {X : Name} {U : Ty} {y : Name} {T : Ty} :
+   ((y, .tm T) :: Γ)[X ↦ U] = (y, .tm T[X ↦ U]) :: Γ[X ↦ U] := rfl
+
+@[simp]
+lemma substCtx_cons_ty {Γ : Context} {X : Name} {U : Ty} {Y : Name} :
+   ((Y, .ty) :: Γ)[X ↦ U] = (Y, .ty) :: Γ[X ↦ U] := rfl
 
 /-
   Substituting a free variable that is not free in the context does nothing.
@@ -56,12 +64,35 @@ lemma substCtx_fresh {Γ : Context} {X : Name} {U : Ty} (h : X ∉ Γ.fv) :
   induction Γ with
   | nil => simp
   | cons head tail ih =>
-    rcases head with ⟨y, T⟩
-    simp only [substCtx_cons, List.cons.injEq, Prod.mk.injEq, true_and]
-    simp only [Context.fv, List.foldr] at *
-    simp_all only [Finset.mem_union, not_or, not_false_eq_true, substTy_fresh, and_self]
+    rcases head with ⟨y, b⟩
+    cases b with
+    | ty =>
+      simp only [substCtx_cons_ty, List.cons.injEq, true_and]
+      apply ih
+      simp [Context.fv] at *
+      aesop
+    | tm T =>
+      simp only [substCtx_cons_tm, List.cons.injEq, Prod.mk.injEq, Binding.tm.injEq, true_and]
+      simp only [Context.fv, List.foldr_cons, Finset.mem_union, not_or] at *
+      constructor
+      · rw [substTy_fresh h.2]
+      · aesop
 
+lemma substCtx_append {Γ₁ Γ₂ : Context} {X : Name} {U : Ty} :
+    (Γ₁ ++ Γ₂)[X ↦ U] = Γ₁[X ↦ U] ++ Γ₂[X ↦ U] := by
+  induction Γ₁ with
+  | nil => simp_all only [List.nil_append, substCtx_nil]
+  | cons head tail ih =>
+    simp only [List.cons_append]
+    rcases head with ⟨y, b⟩
+    cases b with
+    | ty => aesop
+    | tm T => aesop
 
+lemma substCtx_tm_mem {Γ : Context} {x : Name} {T U : Ty} {X : Name}
+    (h : (x, .tm T) ∈ Γ) :
+    (x, .tm T[X ↦ U]) ∈ Γ[X ↦ U] := by
+  exact List.mem_map_of_mem h
 /-
   Well-typed terms are locally closed terms.
 -/
@@ -120,7 +151,7 @@ lemma typing_regularity_wf {Γ t T} (h : Γ ⊢ t ∶ T) : WfContext Γ := by
   | tLam L Γ t T _ ih =>
     have ⟨X, hX⟩ := exists_fresh_name L
     specialize ih X hX
-    assumption
+    exact wf_remove_mid (Γ₁ := []) (Γ₂ := Γ) ih
   | tApp Γ t T₁ T₂ _ _ _ => assumption
 
 end SystemF
