SystemF/Metatheory.lean
@@ -9,42 +9,40 @@ namespace SystemF
   Inserting a new variable into a well-formed context preserves well-formedness,
   as long as the new variable is not free in the existing context.
 -/
-theorem typing_weakening {Γ₁ Γ₂ : Context} {t : Tm} {T U : Ty} {x : Name}
+theorem typing_weakening {Γ₁ Γ₂ : Context} {t : Tm} {T : Ty} {x : Name} {b : Binding}
     (hTyping : (Γ₁ ++ Γ₂) ⊢ t ∶ T)
-    (hWf : WfContext (Γ₁ ++ (x, U) :: Γ₂)) :
-    (Γ₁ ++ (x, U) :: Γ₂) ⊢ t ∶ T := by
+    (hWf : WfContext (Γ₁ ++ (x, b) :: Γ₂)) :
+    (Γ₁ ++ (x, b) :: Γ₂) ⊢ t ∶ T := by
   generalize h : Γ₁ ++ Γ₂ = Γ at hTyping
   induction hTyping generalizing Γ₁ with
   | var Γ x T _ _ _ =>
     subst h
     constructor <;> aesop
   | lam L Γ T₁ T₂ t _ _ ih =>
-    let ctx := (Γ₁ ++ (x, U) :: Γ₂)
+    subst h
+    let ctx := (Γ₁ ++ (x, b) :: Γ₂)
     apply HasType.lam (L ∪ ctx.dom)
     · assumption
     · intro y hy
       have hy₁ : y ∉ L := by aesop
       have hy₂ : y ∉ ctx.dom := by aesop
-      have hWf_new : WfContext ((y, T₁) :: ctx) := by
+      have hWf_new : WfContext ((y, .tm T₁) :: Γ₁ ++ (x, b) :: Γ₂) := by
         constructor <;> assumption
-      simp only [ctx] at hWf_new
-      subst h
-      have heq : (y, T₁) :: Γ₁ ++ Γ₂ = (y, T₁) :: (Γ₁ ++ Γ₂) := by simp
-      have heq' : (y, T₁) :: (Γ₁ ++ (x, U) :: Γ₂) = ((y, T₁) :: Γ₁) ++ (x, U) :: Γ₂ := by simp
-      have : WfContext (((y, T₁) :: Γ₁) ++ (x, U) :: Γ₂) := by
-        rw [← heq']
-        exact hWf_new
-      exact ih y hy₁ this heq
+      exact ih y hy₁ hWf_new rfl
   | app Γ t₁ t₂ T₁ T₂ _ _ ih₁ ih₂ =>
     constructor
     · apply ih₁ hWf h
     · apply ih₂ hWf h
   | tLam L Γ t T _ ih =>
-    let ctx := (Γ₁ ++ (x, U) :: Γ₂)
-    apply HasType.tLam (L ∪ ctx.fv)
+    subst h
+    let ctx := (Γ₁ ++ (x, b) :: Γ₂)
+    apply HasType.tLam (L ∪ ctx.dom)
     intro Y hY
     have hY₁ : Y ∉ L := by aesop
-    exact ih Y hY₁ hWf h
+    have hY₂ : Y ∉ ctx.dom := by aesop
+    have hWf_new : WfContext ((Y, .ty) :: Γ₁ ++ (x, b) :: Γ₂) := by
+      constructor <;> assumption
+    exact ih Y hY₁ hWf_new rfl
   | tApp Γ t T₁ T₂ _ _ ih =>
     constructor
     · apply ih hWf h
@@ -56,8 +54,8 @@ theorem typing_weakening {Γ₁ Γ₂ : Context} {t : Tm} {T U : Ty} {x : Name}
   yields `(x, T[X ↦ U])` in `Γ[X ↦ U]`.
 -/
 theorem substCtx_lookup {Γ : Context} {x : Name} {T U : Ty} {X : Name}
-    (h : (x, T) ∈ Γ) :
-    (x, T[X ↦ U]) ∈ Γ[X ↦ U] := by
+    (h : (x, .tm T) ∈ Γ) :
+    (x, .tm T[X ↦ U]) ∈ Γ[X ↦ U] := by
   induction Γ with
   | nil => simp only [substCtx_nil, List.not_mem_nil]; contradiction
   | cons head tail ih =>
@@ -65,28 +63,38 @@ theorem substCtx_lookup {Γ : Context} {x : Name} {T U : Ty} {X : Name}
     cases h with
     | inl h =>
       subst h
-      simp only [substCtx_cons, List.mem_cons, true_or]
+      simp only [substCtx_cons_tm, List.mem_cons, true_or]
     | inr h =>
       simp_all only [forall_const]
-      cases head
-      simp_all only [substCtx_cons, List.mem_cons, Prod.mk.injEq, or_true]
-
+      rcases head with ⟨y, b⟩
+      cases b with
+      | ty => simp_all only [substCtx_cons_ty, List.mem_cons, Prod.mk.injEq, reduceCtorEq,
+        and_false, or_true]
+      | tm T => simp_all only [substCtx_cons_tm, List.mem_cons, Prod.mk.injEq, Binding.tm.injEq,
+        or_true]
 @[simp]
 lemma substCtx_dom {Γ : Context} {X : Name} {U : Ty} :
     (Γ[X ↦ U]).dom = Γ.dom := by
   induction Γ with
   | nil => simp
   | cons head tail ih =>
-    cases head
-    simp only [substCtx_cons, dom_cons, Finset.singleton_union]
-    rw [ih]
+    rcases head with ⟨y, b⟩
+    cases b with
+    | ty => simp_all only [substCtx_cons_ty, dom_cons, Finset.singleton_union]
+    | tm T => simp_all only [substCtx_cons_tm, dom_cons, Finset.singleton_union]
 
 lemma substCtx_wf {Γ : Context} {X : Name} {U : Ty}
     (hWf : WfContext Γ) (hU : LcTy U) : WfContext (Γ[X ↦ U]) := by
   induction hWf with
   | nil => simp; constructor
-  | cons Γ x T _ _ hLc ih =>
-    simp only [substCtx_cons]
+  | consTy Γ X _ _ ih =>
+    simp only [substCtx_cons_ty]
+    constructor
+    · assumption
+    · simp only [substCtx_dom]
+      assumption
+  | consTm Γ x T _ _ hLc ih =>
+    simp only [substCtx_cons_tm]
     constructor
     · assumption
     · simp only [substCtx_dom]
@@ -96,56 +104,72 @@ lemma substCtx_wf {Γ : Context} {X : Name} {U : Ty}
 /-
   Substitution lemma for types
 -/
-theorem typing_subst_ty {Γ : Context} {t : Tm} {T U : Ty} {X : Name}
-    (hTyping : Γ ⊢ t ∶ T)
+theorem typing_subst_ty {Γ₁ Γ₂ : Context} {t : Tm} {T U : Ty} {X : Name}
+    (hTyping : (Γ₁ ++ (X, .ty) :: Γ₂) ⊢ t ∶ T)
     (hLcTy : LcTy U) :
-    (Γ[X ↦ U]) ⊢ (t[X ↦ U]) ∶ (T[X ↦ U]) := by
-  induction hTyping with
+    (Γ₁[X ↦ U] ++ Γ₂[X ↦ U]) ⊢ (t[X ↦ U]) ∶ (T[X ↦ U]) := by
+  generalize h : Γ₁ ++ (X, .ty) :: Γ₂ = Γ at hTyping
+  induction hTyping generalizing Γ₁ with
   | var Γ x T hWf h₁ h₂ =>
+    subst h
     constructor
-    · exact substCtx_wf hWf hLcTy
-    · exact substCtx_lookup h₁
+    · have := wf_remove_mid hWf
+      have := substCtx_wf this hLcTy (X := X)
+      simp only at this
+      rw [substCtx_append] at this
+      exact this
+    · simp only [List.mem_append, List.mem_cons, Prod.mk.injEq, reduceCtorEq, and_false,
+      false_or] at h₁
+      simp only [List.mem_append]
+      cases h₁ with
+      | inl h =>
+        left
+        apply substCtx_tm_mem
+        assumption
+      | inr h =>
+        right
+        apply substCtx_tm_mem
+        assumption
     · exact substTy_lcTy h₂ hLcTy
   | lam L Γ T₁ T₂ t h₁ h₂ ih =>
+    subst h
     apply HasType.lam (L ∪ {X} ∪ U.fv)
     · exact substTy_lcTy h₁ hLcTy
     · intro y hy
       have hy₁ : y ∉ L := by aesop
-      specialize ih y hy₁
-      -- ((y, substTy X U T₁) :: Γ[X ↦ U]) ⊢ substTmTy X U t⟪$vy⟫ ∶ substTy X U T₂
-      change ((y, T₁[X ↦ U]) :: Γ[X ↦ U]) ⊢ (t[X ↦ U])⟪$vy⟫ ∶ (T₂[X ↦ U])
+      -- ((y, .tm (substTy X U T₁)) :: (Γ₁[X ↦ U] ++ Γ₂[X ↦ U])) ⊢
+      --  substTmTy X U t⟪$vy⟫ ∶ substTy X U T₂
+      change ((y, .tm T₁[X ↦ U]) :: (Γ₁[X ↦ U] ++ Γ₂[X ↦ U])) ⊢ (t[X ↦ U])⟪$vy⟫ ∶ (T₂[X ↦ U])
+      have := ih (Γ₁ := (y, Binding.tm T₁) :: Γ₁) y hy₁ rfl
       rw [openTm_substTmTy_comm_fresh]
-      · exact ih
+      · exact this
       simp [Tm.fvTy]
   | app Γ t₁ t₂ T₁ T₂ _ _ ih₁ ih₂ =>
     simp only [substTmTy_app]
-    constructor
-    · apply ih₁
-    · apply ih₂
+    constructor <;> aesop
   | tLam L Γ t T _ ih =>
+    subst h
     apply HasType.tLam (L ∪ {X} ∪ U.fv)
     intro Y hY
-    -- Γ[X ↦ U] ⊢ substTmTy X U t⟪$TY⟫ ∶ substTy X U T⟪$TY⟫
-    change (Γ[X ↦ U]) ⊢ (t[X ↦ U])⟪$TY⟫ ∶ (T[X ↦ U])⟪$TY⟫
+    -- ((Y, .ty) :: (Γ₁[X ↦ U] ++ Γ₂[X ↦ U])) ⊢ substTmTy X U t⟪$TY⟫ ∶ substTy X U T⟪$TY⟫
+    change ((Y, .ty) :: (Γ₁[X ↦ U] ++ Γ₂[X ↦ U])) ⊢ (t[X ↦ U])⟪$TY⟫ ∶ (T[X ↦ U])⟪$TY⟫
     have hY₁ : Y ∉ L := by aesop
     have hY₂ : X ≠ Y := by aesop
     rw [openTy_substTy_comm hY₂ hLcTy]
     rw [openTmTy_substTmTy_comm hY₂ hLcTy]
-    specialize ih Y hY₁
-    exact ih
+    have := ih (Γ₁ := (Y, .ty) :: Γ₁) Y hY₁ rfl
+    exact this
   | tApp Γ t T₁ T₂ _ _ ih =>
-    simp only [substTmTy_tApp]
     rw [substTy_dist_openTy hLcTy]
     constructor
-    · simp only [subst_all] at ih
-      exact ih
+    · aesop
     · apply substTy_lcTy <;> assumption
 
 theorem typing_subst_tm {Γ₁ Γ₂ : Context} {t u : Tm} {T U : Ty} {x : Name}
-    (hTyping : (Γ₁ ++ (x, U) :: Γ₂) ⊢ t ∶ T)
+    (hTyping : (Γ₁ ++ (x, .tm U) :: Γ₂) ⊢ t ∶ T)
     (hSubstTyping : (Γ₁ ++ Γ₂) ⊢ u ∶ U) :
     (Γ₁ ++ Γ₂) ⊢ (t[x ↦ u]) ∶ T := by
-  generalize h : Γ₁ ++ (x, U) :: Γ₂ = Γ at hTyping
+  generalize h : Γ₁ ++ (x, .tm U) :: Γ₂ = Γ at hTyping
   induction hTyping generalizing Γ₁ with
   | var Γ x' T _ _ _ =>
     simp only [substTm_fvar, beq_iff_eq]
@@ -153,7 +177,8 @@ theorem typing_subst_tm {Γ₁ Γ₂ : Context} {t u : Tm} {T U : Ty} {x : Name}
     · simp_all only
       rename_i hWf mem _ _
       subst h
-      have : T = U := wf_lookup_mid hWf mem
+      have : Binding.tm T = Binding.tm U := wf_lookup_mid hWf mem
+      have : T = U := by injection this
       rw [this]
       assumption
     · subst h
@@ -171,16 +196,16 @@ theorem typing_subst_tm {Γ₁ Γ₂ : Context} {t u : Tm} {T U : Ty} {x : Name}
       have hy₂ : y ≠ x := by aesop
       have hy₃ : y ∉ Context.dom (Γ₁ ++ Γ₂) := by aesop
       rw [openTm_substTm_comm_of_neq hy₂ hLCu]
-      have : ((y, T₁) :: Γ₁ ++ Γ₂) ⊢ u ∶ U := by
-        have := typing_weakening (Γ₁ := []) (Γ₂ := Γ₁ ++ Γ₂) (x := y) (U := T₁) hSubstTyping
+      have : ((y, .tm T₁) :: Γ₁ ++ Γ₂) ⊢ u ∶ U := by
+        have := typing_weakening (Γ₁ := []) (Γ₂ := Γ₁ ++ Γ₂) (x := y) (b := .tm T₁) hSubstTyping
         simp only [List.nil_append] at this
         apply this
         constructor
         · exact typing_regularity_wf hSubstTyping
         · exact hy₃
         · assumption
-      -- Γ₁ ++ (x, U) :: Γ₂ = (y, T₁) :: (Γ₁ ++ (x, U) :: Γ₂)
-      exact @ih y hy₁ ((y, T₁) :: Γ₁) this (by aesop)
+      -- Γ₁ ++ (x, .tm U) :: Γ₂ = (y, .tm T₁) :: (Γ₁ ++ (x, .tm U) :: Γ₂)
+      exact @ih y hy₁ ((y, .tm T₁) :: Γ₁) this (by aesop)
   | app Γ t₁ t₂ T₁ T₂ _ _ ih₁ ih₂ =>
     subst h
     simp only [substTm_app]
@@ -193,14 +218,17 @@ theorem typing_subst_tm {Γ₁ Γ₂ : Context} {t u : Tm} {T U : Ty} {x : Name}
       · rfl
   | tLam L Γ t T _ ih =>
     simp only [substTm_tLam]
-    apply HasType.tLam (L ∪ {x} ∪ (Context.fv Γ))
+    apply HasType.tLam (L ∪ Context.dom Γ)
     intro Y hY
     have hLCu : LcTm u := typing_regularity_tm hSubstTyping
     have hY₁ : Y ∉ L := by aesop
+    have hY₂ : Y ∉ Context.dom (Γ₁ ++ Γ₂) := by aesop
     rw [←openTmTy_substTm_comm hLCu]
+    rw [←List.cons_append]
     apply ih
     · assumption
-    · assumption
+    · have : WfContext (Γ₁ ++ Γ₂) := typing_regularity_wf hSubstTyping
+      exact typing_weakening (Γ₁ := []) hSubstTyping (by constructor <;> assumption)
     · aesop
   | tApp Γ t T₁ T₂ _ _ ih =>
     constructor
@@ -246,7 +274,7 @@ theorem preservation {Γ : Context} {t t' : Tm} {T : Ty}
         rw [←substTy_openTy_var hX₂]
         rw [←substTmTy_openTmTy_var hX₃]
         have := hBody X hX₁
-        have := typing_subst_ty (X := X) (T := T₁⟪$TX⟫) (U := T) this (by assumption)
+        have := typing_subst_ty (Γ₁ := []) this (by assumption)
         rw [substCtx_fresh hX₄] at this
         exact this
 
